Rename AES create_ctx to state_alloca

code/aes/Hacl.AES_128.CTR32.NI.fst
@@ -20,7 +20,7 @@ let aes_ctx = aes_ctx MAES Spec.AES128
 let skey = skey Spec.AES128
 
 inline_for_extraction noextract
-val create_ctx: unit ->
+val state_alloca: unit ->
   StackInline aes_ctx
   (requires (fun h -> True))
   (ensures  (fun h0 f h1 -> live h1 f /\
@@ -28,7 +28,7 @@ val create_ctx: unit ->
     (elem_zero MAES))))
 
 inline_for_extraction noextract
-let create_ctx () = create_ctx MAES Spec.AES128
+let state_alloca () = create_ctx MAES Spec.AES128
 
 inline_for_extraction
 val state_malloc:
